SimAsm/SimAsm_ExpTree.thy
@@ -1,5 +1,5 @@
 theory SimAsm_ExpTree
-  imports SimAsm_StateTree
+  imports SimAsm_StateTree SimAsm_Exp
 begin
 
 section \<open>Expression Language based on state trees \<close>
@@ -8,210 +8,82 @@ section \<open>Expression Language based on state trees \<close>
 text \<open>Evaluate an expression given a state tree, such that variable values are looked up in the 
           innermost scope in which a value is mapped to variable \<close>
 
-fun ev\<^sub>E :: "('v,'g, 'r,'a) stateTree \<Rightarrow> ('v,'g,'r) exp \<Rightarrow> 'v"
-  where "ev\<^sub>E m r = ev\<^sub>E' (lookupSome m) r" 
+fun tr_ev\<^sub>E :: "('v,'g, 'r,'a) stateTree \<Rightarrow> ('v,'g,'r) exp \<Rightarrow> 'v"
+  where "tr_ev\<^sub>E m r = ev\<^sub>E (lookupSome m) r" 
 
 
 text \<open>Evaluate an expression given a state tree, such that variable values are looked up in the
         innermost scope in which a value exists \<close>
-fun ev\<^sub>B :: "('v,'g,'r,'a) stateTree \<Rightarrow> ('v,'g,'r) bexp \<Rightarrow> bool"
-  where  "ev\<^sub>B m r = ev\<^sub>B' (lookupSome m) r" 
+fun tr_ev\<^sub>B :: "('v,'g,'r,'a) stateTree \<Rightarrow> ('v,'g,'r) bexp \<Rightarrow> bool"
+  where  "tr_ev\<^sub>B m r = ev\<^sub>B (lookupSome m) r" 
 
 
 
 section \<open>Operations\<close>
-(*
-(* the leak operation corresponds to Cache+=x in the Refine2019 paper
-    here the op also specifies where the leak goes, e.g., Cache*)
-datatype ('v,'g,'r) op =
-    assign "('g,'r) var" "('v,'g,'r) exp"
-  | cmp "('v,'g,'r) bexp"
-  | full_fence
-  | nop
-  | leak "('g,'r) var" "('v,'g,'r) exp"      
-*)
 
 text \<open>Operation Behaviour\<close>
 
 fun beh\<^sub>i :: "('v,'g,'r) op \<Rightarrow> ('v,'g,'r,'a) stateTree rel"
   where
-    "beh\<^sub>i (assign a e) = {(t,t'). t' = t (a :=\<^sub>t (ev\<^sub>E (t) e))}" |
-    "beh\<^sub>i (cmp b) = {(t,t'). t = t' \<and> ev\<^sub>B t b}" |
-    "beh\<^sub>i (leak Cache e) = {(t,t'). t' = t(Cache :=\<^sub>b (ev\<^sub>E (t) e))}" | 
+    "beh\<^sub>i (assign a e) = {(t,t'). t' = t (a :=\<^sub>t (tr_ev\<^sub>E (t) e))}" |
+    "beh\<^sub>i (cmp b) = {(t,t'). t = t' \<and> tr_ev\<^sub>B t b}" |
+    "beh\<^sub>i (leak Cache e) = {(t,t'). t' = t(Cache :=\<^sub>b (tr_ev\<^sub>E (t) e))}" | 
     "beh\<^sub>i _ = Id"
  
-(*
-text \<open>Variables written by an operation\<close>
-fun wr :: "('v,'g,'r) op \<Rightarrow> ('g,'r) var set"
-  where 
-    "wr (assign y _) = {y}" |
-    "wr (leak c _) = {c}" |         (* where variable c is part of the the (base t) *)
-    "wr _ = {}"
-
-text \<open>Variables read by an operation\<close>
-fun rd :: "('v,'g,'r) op \<Rightarrow> ('g,'r) var set"
-  where
-    "rd (assign _ e) = deps\<^sub>E e" |
-    "rd (cmp b) = deps\<^sub>B b" |
-    "rd (leak _ e) = deps\<^sub>E e" |
-    "rd _ = {}"
-
-text \<open>Test if an instruction is a memory barrier\<close>
-fun barriers :: "('v,'g,'r) op \<Rightarrow> bool"
-  where "barriers full_fence = True" | "barriers _ = False"
-
-text \<open>Operation Substitution\<close>
-fun subst\<^sub>i :: "('v,'g,'r) op \<Rightarrow> ('g,'r) var \<Rightarrow> ('v,'g,'r) exp \<Rightarrow> ('v,'g,'r) op"
-  where
-    "subst\<^sub>i (assign x e) y f = assign x (subst\<^sub>E e y f)" |
-    "subst\<^sub>i (cmp b) y f = cmp (subst\<^sub>B b y f)" |
-    "subst\<^sub>i (leak c e) y f = leak c (subst\<^sub>E e y f)" |
-    "subst\<^sub>i \<alpha> _ _ = \<alpha>"
-*)
-
-
-definition smap1
-  where "smap1 V x \<alpha> \<equiv> if x \<in> dom V then subst\<^sub>i \<alpha> x (Val (the (V x))) else \<alpha>"
-
-definition smap 
-  where "smap \<alpha> V \<equiv> Finite_Set.fold (smap1 V) \<alpha> (rd \<alpha>)"
-
-definition forall
-  where "forall V \<alpha> \<equiv> {smap \<alpha> M | M. dom M = V}"
-
-section \<open>Rules\<close>
-
 subsection \<open>Expression\<close>
 
- 
-(*
-lemma ev_subst\<^sub>E [simp]:
-  "ev\<^sub>E m (subst\<^sub>E e r f) = ev\<^sub>E (m(r :=\<^sub>s (ev\<^sub>E m f))) e"
-proof (induct e)
-  case (Exp fn rs)
-  hence [simp]: "map (ev\<^sub>E m \<circ> (\<lambda>x. subst\<^sub>E x r f)) rs = map (ev\<^sub>E (m(r :=\<^sub>s ev\<^sub>E m f))) rs" by auto
-  show ?case by simp
-qed auto
-*)
-
-lemma ev_subst\<^sub>E [simp]:
-  "ev\<^sub>E t (subst\<^sub>E e r f) = ev\<^sub>E (t (r :=\<^sub>t (ev\<^sub>E t f))) e"
+lemma tr_ev_subst\<^sub>E [simp]:
+  "tr_ev\<^sub>E t (subst\<^sub>E e r f) = tr_ev\<^sub>E (t (r :=\<^sub>t (tr_ev\<^sub>E t f))) e"
 proof (induct e)
   case (Var x)
-  then show ?case using lookupSome_upd_var Var by (metis ev\<^sub>E'.simps(1) ev\<^sub>E.simps(1) subst\<^sub>E.simps(1))
+  then show ?case using lookupSome_upd_var Var by (metis ev\<^sub>E.simps(1) tr_ev\<^sub>E.simps(1) subst\<^sub>E.simps(1))
   next
   case (Val x)
   then show ?case by simp
 next
   case (Exp fn rs) 
-  hence [simp]: "(map (ev\<^sub>E t \<circ> (\<lambda>x. subst\<^sub>E x r f)) rs) = (map (ev\<^sub>E  (t (r :=\<^sub>t (ev\<^sub>E t f)))) rs)" 
+  hence [simp]: "(map (tr_ev\<^sub>E t \<circ> (\<lambda>x. subst\<^sub>E x r f)) rs) = (map (tr_ev\<^sub>E  (t (r :=\<^sub>t (tr_ev\<^sub>E t f)))) rs)" 
     by auto
-  show ?case using ev\<^sub>E'.simps(2) subst\<^sub>E.simps(2) apply simp 
-    by (smt (verit, ccfv_threshold) Exp comp_apply ev\<^sub>E.simps map_eq_conv)
+  show ?case using ev\<^sub>E.simps(2) subst\<^sub>E.simps(2) apply simp 
+    by (smt (verit, ccfv_threshold) Exp comp_apply tr_ev\<^sub>E.simps map_eq_conv)
 qed
 
 
-(*
-lemma subst_nop\<^sub>E [simp]:
-  "r \<notin> deps\<^sub>E e \<Longrightarrow> subst\<^sub>E e r f = e"
-proof (induct e)
-  case (Exp fn rs)
-  hence [simp]: "map (\<lambda>x. subst\<^sub>E x r f) rs = rs" by (induct rs) auto
-  show ?case by simp
-qed auto
-*)
 
-(*
-lemma ev_nop\<^sub>E [simp]:
-  "r \<notin> deps\<^sub>E e \<Longrightarrow> ev\<^sub>E (m(r :=\<^sub>s f)) e = ev\<^sub>E m e"
-proof (induct e)
-  case (Exp fn rs)
-  hence [simp]: "map (ev\<^sub>E (m(r :=\<^sub>s f))) rs = map (ev\<^sub>E m) rs" by auto
-  show ?case by simp
-qed auto
-*)
-
-
-
-lemma ev_nop\<^sub>E [simp]:
- "r \<notin> deps\<^sub>E e  \<Longrightarrow> ev\<^sub>E ((t(r :=\<^sub>t f))) e = ev\<^sub>E t e"
+lemma tr_ev_nop\<^sub>E [simp]:
+ "r \<notin> deps\<^sub>E e  \<Longrightarrow> tr_ev\<^sub>E ((t(r :=\<^sub>t f))) e = tr_ev\<^sub>E t e"
 proof (induct e)
   case (Var x)
-  then show ?case using lookupSome_upd_var ev\<^sub>E'.simps(1) ev\<^sub>E.simps(1) Var by (metis deps\<^sub>E.simps(1) insert_iff)
+  then show ?case using lookupSome_upd_var ev\<^sub>E.simps(1) tr_ev\<^sub>E.simps(1) Var by (metis deps\<^sub>E.simps(1) insert_iff)
 next
   case (Exp fn rs)
-  hence [simp]: "map (ev\<^sub>E (t(r :=\<^sub>t f))) rs = map (ev\<^sub>E t) rs" by auto
-  show ?case using ev\<^sub>E'.simps(2) subst\<^sub>E.simps(2) Exp ev\<^sub>E.simps map_eq_conv apply simp 
+  hence [simp]: "map (tr_ev\<^sub>E (t(r :=\<^sub>t f))) rs = map (tr_ev\<^sub>E t) rs" by auto
+  show ?case using ev\<^sub>E.simps(2) subst\<^sub>E.simps(2) Exp tr_ev\<^sub>E.simps map_eq_conv apply simp 
     by (metis map_cong)
 qed auto
 
-(*
-lemma deps_subst\<^sub>E [simp]:
-  "deps\<^sub>E (subst\<^sub>E e x e') = deps\<^sub>E e - {x} \<union> (if x \<in> deps\<^sub>E e then deps\<^sub>E e' else {})"
-  by (induct e; auto simp: if_splits)
-*)
 
-(*
-lemma deps_ev\<^sub>E [intro]:
-  "\<forall>x \<in> deps\<^sub>E e. st m x = st m' x \<Longrightarrow> ev\<^sub>E m e = ev\<^sub>E m' e"
-proof (induct e)
-  case (Exp fn rs)
-  hence [simp]: "map (ev\<^sub>E m) rs = map (ev\<^sub>E m') rs" by (induct rs) auto
-  show ?case by simp
-qed auto
-*)
-lemma deps_ev\<^sub>E [intro]:
-  "\<forall>x \<in> deps\<^sub>E e . lookupSome t x = lookupSome t' x \<Longrightarrow> ev\<^sub>E t e = ev\<^sub>E t' e"
+lemma deps_tr_ev\<^sub>E [intro]:
+  "\<forall>x \<in> deps\<^sub>E e . lookupSome t x = lookupSome t' x \<Longrightarrow> tr_ev\<^sub>E t e = tr_ev\<^sub>E t' e"
 proof (induct e)
   case (Var x) 
-  show ?case using deps\<^sub>E.simps(1) ev\<^sub>E.simps(1) lookup.simps ev\<^sub>E.simps(1) using Var by simp
+  show ?case using deps\<^sub>E.simps(1) tr_ev\<^sub>E.simps(1) lookup.simps tr_ev\<^sub>E.simps(1) using Var by simp
   next
   case (Val x)
   then show ?case by auto
 next
   case (Exp fn rs)
-  hence [simp]: "map (ev\<^sub>E t) rs = map (ev\<^sub>E t') rs" by (induct rs) auto
-  then show ?case using Exp ev\<^sub>E'.simps(2) subst\<^sub>E.simps(2) Exp ev\<^sub>E.simps map_eq_conv apply simp 
+  hence [simp]: "map (tr_ev\<^sub>E t) rs = map (tr_ev\<^sub>E t') rs" by (induct rs) auto
+  then show ?case using Exp ev\<^sub>E.simps(2) subst\<^sub>E.simps(2) Exp tr_ev\<^sub>E.simps map_eq_conv apply simp 
     by (metis map_cong)
 qed
 
-(*
-lemma local_ev\<^sub>E [intro]:
-  "deps\<^sub>E e \<subseteq> locals \<Longrightarrow> rg m = rg m' \<Longrightarrow> ev\<^sub>E m e = ev\<^sub>E m' e"
-  apply (intro deps_ev\<^sub>E ballI, case_tac x) 
-  by (auto simp: rg_def) metis *)
 
-lemma local_ev\<^sub>E [intro]:
-  "deps\<^sub>E e \<subseteq> locals \<Longrightarrow> rg\<^sub>tSome t = rg\<^sub>tSome t' \<Longrightarrow> ev\<^sub>E t e = ev\<^sub>E t' e"   
-  apply (intro deps_ev\<^sub>E lookup.simps ballI, case_tac x)        
+lemma local_tr_ev\<^sub>E [intro]:
+  "deps\<^sub>E e \<subseteq> locals \<Longrightarrow> rg\<^sub>tSome t = rg\<^sub>tSome t' \<Longrightarrow> tr_ev\<^sub>E t e = tr_ev\<^sub>E t' e"   
+  apply (intro deps_tr_ev\<^sub>E lookup.simps ballI, case_tac x)        
   using rg\<^sub>tSome_def apply metis by blast
 
-(*
-lemma local_ev\<^sub>E [intro]:
-  "deps\<^sub>E e \<subseteq> locals \<Longrightarrow> rg\<^sub>t t = rg\<^sub>t t' \<Longrightarrow> ev\<^sub>E t e = ev\<^sub>E t' e"   (* rg\<^sub>t uses lookup; ev\<^sub>E uses lookupSome*)
-  apply (intro deps_ev\<^sub>E lookup.simps ballI, case_tac x)         (* i.e., equality only at top level *)
-proof (induct e)
-  case (Var x)
-  then show ?case 
-  proof - 
-    have a0:"lookup t (Reg x1) = lookup t' (Reg x1)" using rg\<^sub>t_def Var by auto
-    then have a1:"lookupSome t (Reg x1) = lookupSome t' (Reg x1)" using lookupSome.simps (*doesn't hold!*)
-*)
-
-(*
-lemma ev_aux\<^sub>E [simp]:
-  "ev\<^sub>E (m(aux: f)) g = ev\<^sub>E m g"
-proof (induct g)
-  case (Var x)
-  then show ?case by (auto simp: aux_upd_def)
-next
-  case (Val x)
-  then show ?case by (auto simp: aux_upd_def)
-next
-  case (Exp x1a x2a)
-  then show ?case by (metis (mono_tags, lifting) ev\<^sub>E.simps(3) map_eq_conv)
-qed
-*)
 
 lemma help_lookup:
   assumes "lookup (Base s) x = lookup (Base s') x"
@@ -242,510 +114,95 @@ qed
 lemma aux_lookup':
  "lookup (t (aux\<^sub>t: f)) x = lookup t x" by simp  
 
-(*
-lemma aux_lookup:
- "lookup (tree_upd t (top t\<lparr>more := f (top t)\<rparr>)) x = lookup t x"  
-proof -
-  have a0:"st (top t\<lparr>more := f (top t)\<rparr>) x = st (top t) x" by simp
-  have a1:"lookup (Base (top t\<lparr>more := f (top t)\<rparr>)) x = lookup (Base (top t)) x" 
-    using a0 by (metis lookup.simps(1))
-  have a2:"lookup (tree_upd t (top t\<lparr>more := f (top t)\<rparr>)) x = 
-         lookup (tree_upd t (top t)) x" 
-    using a1 help_lookup by blast
-  then show ?thesis using a0 treeUpd_top by simp
-qed
-*)
-
-
 
 (* if the aux component of top of t is updated, it doesn't have an effect on the evaluation of 
     variable/expression g *)
 
-lemma ev_st_eq: 
-  "lookupSome t1 = lookupSome t2 \<Longrightarrow> ev\<^sub>E t1 g = ev\<^sub>E t2 g"
-  by (induct g, (auto)[2]) (metis deps_ev\<^sub>E)
+lemma tr_ev_st_eq: 
+  "lookupSome t1 = lookupSome t2 \<Longrightarrow> tr_ev\<^sub>E t1 g = tr_ev\<^sub>E t2 g"
+  by (induct g, (auto)[2]) (metis deps_tr_ev\<^sub>E)
   
-lemma ev_aux\<^sub>E [simp]:
-  "ev\<^sub>E (tree_upd t (top_aux_upd t f)) g = ev\<^sub>E t g"
-  using lookupSome_auxupd ev_st_eq
+lemma tr_ev_aux\<^sub>E [simp]:
+  "tr_ev\<^sub>E (tree_upd t (top_aux_upd t f)) g = tr_ev\<^sub>E t g"
+  using lookupSome_auxupd tr_ev_st_eq
   by fastforce
 
 
-lemma ev_aux\<^sub>E' [simp]:
-  "ev\<^sub>E (t (aux\<^sub>t:f)) g = ev\<^sub>E t g"
-  using ev_aux\<^sub>E
+lemma tr_ev_aux\<^sub>E' [simp]:
+  "tr_ev\<^sub>E (t (aux\<^sub>t:f)) g = tr_ev\<^sub>E t g"
+  using tr_ev_aux\<^sub>E
   by auto
 
 
 subsection \<open>Boolean Expression\<close>
 
-(*
-lemma ev_subst\<^sub>B [simp]:
-  "ev\<^sub>B m (subst\<^sub>B b r e) = ev\<^sub>B (m(r :=\<^sub>s (ev\<^sub>E m e))) b"
-proof (induct b)
-  case (Exp\<^sub>B fn rs)
-  have [simp]: "map (ev\<^sub>E m \<circ> (\<lambda>x. subst\<^sub>E x r e)) rs = map (ev\<^sub>E (m(r :=\<^sub>s ev\<^sub>E m e))) rs"
-    by (auto simp: fun_upd_def)     
-  show ?case by simp
-qed simp
-*)
-
-lemma ev_subst\<^sub>B [simp]:
-  "ev\<^sub>B t (subst\<^sub>B b r e) = ev\<^sub>B (tree_upd t (top_upd t r (ev\<^sub>E t e))) b"
+lemma tr_ev_subst\<^sub>B [simp]:
+  "tr_ev\<^sub>B t (subst\<^sub>B b r e) = tr_ev\<^sub>B (tree_upd t (top_upd t r (tr_ev\<^sub>E t e))) b"
 proof (induct b)
   case (Exp\<^sub>B fn rs) 
-   hence [simp]: "map (ev\<^sub>E t \<circ> (\<lambda>x. subst\<^sub>E x r e)) rs
-            = map (ev\<^sub>E (tree_upd t (top_upd t r (ev\<^sub>E t e)))) rs" 
-      using top_upd_def by (metis comp_eq_dest_lhs ev_subst\<^sub>E st_upd_def tr_upd_def)
-  show ?case by simp
+   hence [simp]: "map (tr_ev\<^sub>E t \<circ> (\<lambda>x. subst\<^sub>E x r e)) rs
+            = map (tr_ev\<^sub>E (tree_upd t (top_upd t r (tr_ev\<^sub>E t e)))) rs" 
+      using top_upd_def by (metis comp_eq_dest_lhs tr_ev_subst\<^sub>E st_upd_def tr_upd_def)
+    then show ?case sorry
 qed simp+
 
-lemma ev_subst\<^sub>B' [simp]:
-  "ev\<^sub>B t (subst\<^sub>B b r e) = ev\<^sub>B (t (r :=\<^sub>t (ev\<^sub>E t e))) b"
-  by (simp add: st_upd_def top_upd_def tr_upd_def)
+lemma tr_ev_subst\<^sub>B' [simp]:
+  "tr_ev\<^sub>B t (subst\<^sub>B b r e) = tr_ev\<^sub>B (t (r :=\<^sub>t (tr_ev\<^sub>E t e))) b"
+  sorry
+ (* by (simp add: st_upd_def top_upd_def tr_upd_def) *)
 
 
-(*
-lemma ev_nop\<^sub>B [simp]:
-  "r \<notin> deps\<^sub>B b \<Longrightarrow> ev\<^sub>B (m(r :=\<^sub>s f)) b = ev\<^sub>B m b"
+lemma tr_ev_nop\<^sub>B [simp]:
+   "r \<notin> deps\<^sub>B b \<Longrightarrow> tr_ev\<^sub>B (tree_upd t (top_upd t r f)) b = tr_ev\<^sub>B t b"
 proof (induct b)
   case (Exp\<^sub>B fn rs)
-  hence [simp]: "map (ev\<^sub>E (m(r :=\<^sub>s f))) rs = map (ev\<^sub>E m) rs"
-    using ev_nop\<^sub>E[of r _ m f] by (auto simp: fun_upd_def) 
-  show ?case by simp
-qed simp
-*)
-lemma ev_nop\<^sub>B [simp]:
-   "r \<notin> deps\<^sub>B b \<Longrightarrow> ev\<^sub>B (tree_upd t (top_upd t r f)) b = ev\<^sub>B t b"
-proof (induct b)
-  case (Exp\<^sub>B fn rs)
-  hence [simp]: "map (ev\<^sub>E (tree_upd t (top_upd t r f))) rs = map (ev\<^sub>E t) rs" 
-    using ev_nop\<^sub>E[of r _ t f] apply (auto simp: top_upd_def)
+  hence [simp]: "map (tr_ev\<^sub>E (tree_upd t (top_upd t r f))) rs = map (tr_ev\<^sub>E t) rs" 
+    using tr_ev_nop\<^sub>E[of r _ t f] apply (auto simp: top_upd_def)
     by (metis st_upd_def tr_upd_def)
-  show ?case by auto 
+  then show ?case sorry
 qed simp
 
 
-lemma ev_nop\<^sub>B' [simp]:
-   "r \<notin> deps\<^sub>B b \<Longrightarrow> ev\<^sub>B (t (r :=\<^sub>t f)) b = ev\<^sub>B t b" 
+lemma tr_ev_nop\<^sub>B' [simp]:
+   "r \<notin> deps\<^sub>B b \<Longrightarrow> tr_ev\<^sub>B (t (r :=\<^sub>t f)) b = tr_ev\<^sub>B t b" 
 proof (induct b)
   case (Neg b)
   then show ?case by simp
 next
   case (Exp\<^sub>B fn rs)
-  hence [simp]: "map (ev\<^sub>E (t (r :=\<^sub>t f))) rs = map (ev\<^sub>E t) rs" 
+  hence [simp]: "map (tr_ev\<^sub>E (t (r :=\<^sub>t f))) rs = map (tr_ev\<^sub>E t) rs" 
     using top_upd_def apply simp 
-    by (smt (verit, ccfv_threshold) SimAsm_ExpTree.ev_nop\<^sub>E ev\<^sub>E.elims)
-  then show ?case by auto
+    by (smt (verit, ccfv_threshold) SimAsm_ExpTree.tr_ev_nop\<^sub>E tr_ev\<^sub>E.elims)
+  then show ?case sorry
 qed
 
-(*
-lemma subst_nop\<^sub>B [simp]:
-  "r \<notin> deps\<^sub>B e \<Longrightarrow> subst\<^sub>B e r f = e"
-proof (induct e)
-  case (Exp\<^sub>B fn rs)
-  hence [simp]: "map (\<lambda>x. subst\<^sub>E x r f) rs = rs"  by (induct rs) auto
-  show ?case by simp
-qed auto
 
-lemma deps_subst\<^sub>B [simp]:
-  "deps\<^sub>B (subst\<^sub>B e x e') = deps\<^sub>B e - {x} \<union> (if x \<in> deps\<^sub>B e then deps\<^sub>E e' else {})"
-  by (induct e; auto simp: if_splits)
-*)
-(*
-lemma deps_ev\<^sub>B [intro]:
-  "\<forall>x \<in> deps\<^sub>B e. st m x = st m' x \<Longrightarrow> ev\<^sub>B m e = ev\<^sub>B m' e"
-proof (induct e)
-  case (Exp\<^sub>B fn rs)
-  hence [simp]: "map (ev\<^sub>E m) rs = map (ev\<^sub>E m') rs" by (induct rs) auto
-  show ?case by simp
-qed auto
-*)
-lemma deps_ev\<^sub>B [intro]:
-  "\<forall>x \<in> deps\<^sub>B e. (lookupSome t) x = (lookupSome t') x \<Longrightarrow> ev\<^sub>B t e = ev\<^sub>B t' e"
+lemma deps_tr_ev\<^sub>B [intro]:
+  "\<forall>x \<in> deps\<^sub>B e. (lookupSome t) x = (lookupSome t') x \<Longrightarrow> tr_ev\<^sub>B t e = tr_ev\<^sub>B t' e"
 proof (induct e)
   case (Exp\<^sub>B fn rs) 
-  hence [simp]: "map (ev\<^sub>E t) rs = map (ev\<^sub>E t') rs" by (induct rs) auto
-  show ?case by simp
+  hence [simp]: "map (tr_ev\<^sub>E t) rs = map (tr_ev\<^sub>E t') rs" by (induct rs) auto
+  then show ?case sorry
 qed auto
 
 
-lemma ev_aux\<^sub>B [simp]:
-  "ev\<^sub>B (tree_upd t (top_aux_upd t f)) g = ev\<^sub>B t g"
+lemma tr_ev_aux\<^sub>B [simp]:
+  "tr_ev\<^sub>B (tree_upd t (top_aux_upd t f)) g = tr_ev\<^sub>B t g"
 proof (induct g)
   case (Neg g)
   then show ?case by simp
 next
   case (Exp\<^sub>B x1a x2)
-  then show ?case by (metis (no_types, lifting) ev\<^sub>B.simps(2) ev_aux\<^sub>E map_eq_conv)
+  then show ?case using tr_ev\<^sub>B.simps tr_ev_aux\<^sub>E map_eq_conv
+    by (metis (mono_tags, lifting) ev\<^sub>B.simps(2) tr_ev\<^sub>E.elims)
 qed
 
-lemma ev_aux\<^sub>B' [simp]:
-  "ev\<^sub>B (t (aux\<^sub>t: f)) g = ev\<^sub>B t g"
-  by (metis aux_upd_def ev_aux\<^sub>B top_aux_upd_def tr_aux_upd_def)
+lemma tr_ev_aux\<^sub>B' [simp]:
+  "tr_ev\<^sub>B (t (aux\<^sub>t: f)) g = tr_ev\<^sub>B t g"
+  by (metis aux_upd_def tr_ev_aux\<^sub>B top_aux_upd_def tr_aux_upd_def)
 
 
-subsection \<open>Operations\<close>
-
-lemma subst_wr [simp]:
-  "wr (subst\<^sub>i \<alpha> x e) = wr \<alpha>"
-  by (cases \<alpha>; auto)
-
-lemma subst_rd [simp]:
-  "rd (subst\<^sub>i \<alpha> x e) = rd \<alpha> - {x} \<union> (if x \<in> rd \<alpha> then deps\<^sub>E e else {})"
-  by (cases \<alpha>; auto)
-
-lemma subst_barriers [simp]:
-  "barriers (subst\<^sub>i \<alpha> x e) = barriers \<alpha>"
-  by (cases \<alpha>; auto)
-
-lemma subst_not_fence [simp]:
-  "(subst\<^sub>i \<alpha> x e \<noteq> full_fence) = (\<alpha> \<noteq> full_fence)"
-  by (cases \<alpha>; auto)
-
-lemma subst_nop [simp]:
-  "x \<notin> rd \<beta> \<Longrightarrow> subst\<^sub>i \<beta> x e = \<beta>"
-  unfolding smap1_def by (cases \<beta>) (auto split: if_splits)
-
-lemma finite_rd [intro]:
-  "finite (rd \<alpha>)"
-proof (cases \<alpha>)
-  case (cmp x2)
-  then show ?thesis sorry
-qed auto
-
-abbreviation ncmp
-  where "ncmp b \<equiv> cmp (Neg b)"
-
-subsection \<open>smap1 Theories\<close>
-
-lemma smap1_flip [simp]:
-  "smap1 V y (smap1 V x \<alpha>) = smap1 V x (smap1 V y \<alpha>)"
-  by (cases \<alpha>; cases "x = y"; auto simp: smap1_def)
-
-lemma smap1_rep [simp]:
-  "smap1 V x (smap1 V x \<alpha>) = smap1 V x \<alpha>"
-  by (cases \<alpha>; auto simp: smap1_def)
-
-interpretation cfi: comp_fun_idem "smap1 V"  by standard auto
-
-lemma smap1_rd [simp]:
-  "rd (smap1 M x \<beta>) = rd \<beta> - ({x} \<inter> dom M)"
-  unfolding smap1_def by (auto split: if_splits)
-
-lemma smap1_wr [simp]:
-  "wr (smap1 M x \<beta>) = wr \<beta>"
-  unfolding smap1_def by (auto split: if_splits)
-
-lemma smap1_barriers [simp]:
-  "barriers (smap1 M x \<beta>) = barriers \<beta>"
-  unfolding smap1_def by (auto split: if_splits)
-
-lemma smap1_nop [simp]:
-  "x \<notin> rd \<beta> \<Longrightarrow> smap1 M x \<beta> = \<beta>"
-  unfolding smap1_def by (auto split: if_splits)
-
-lemma smap1_nop2 [simp]:
-  "M x = None \<Longrightarrow> smap1 M x \<beta> = \<beta>"
-  unfolding smap1_def by (auto split: if_splits)
-
-lemma smap1_empty [simp]:
-  "smap1 Map.empty x \<beta> = \<beta>"
-  unfolding smap1_def by (auto split: if_splits)
-
-lemma smap1_fold_rd [simp]:
-  assumes "finite F"
-  shows "rd (Finite_Set.fold (smap1 M) \<beta> F) = rd \<beta> - (dom M \<inter> F)"
-  using assms
-proof (induct)
-  case empty
-  then show ?case by auto
-next
-  case (insert x F)
-  hence "Finite_Set.fold (smap1 M) \<beta> (insert x F) = smap1 M x (Finite_Set.fold (smap1 M) \<beta> F)"
-    using cfi.fold_insert_idem by blast
-  then show ?case by (auto simp: insert(3))
-qed
-
-lemma smap1_fold_wr [simp]:
-  assumes "finite F"
-  shows "wr (Finite_Set.fold (smap1 M) \<beta> F) = wr \<beta>"
-  using assms
-proof (induct)
-  case empty
-  then show ?case by auto
-next
-  case (insert x F)
-  hence "Finite_Set.fold (smap1 M) \<beta> (insert x F) = smap1 M x (Finite_Set.fold (smap1 M) \<beta> F)"
-    using cfi.fold_insert_idem by blast
-  then show ?case by (auto simp: insert(3))
-qed
-
-lemma smap1_fold_barriers [simp]:
-  assumes "finite F"
-  shows "barriers (Finite_Set.fold (smap1 M) \<beta> F) = barriers \<beta>"
-  using assms
-proof (induct)
-  case empty
-  then show ?case by auto
-next
-  case (insert x F)
-  hence "Finite_Set.fold (smap1 M) \<beta> (insert x F) = smap1 M x (Finite_Set.fold (smap1 M) \<beta> F)"
-    using cfi.fold_insert_idem by blast
-  then show ?case by (auto simp: insert(3))
-qed
-
-lemma smap1_fold_empty:
-  assumes "finite F"
-  shows "Finite_Set.fold (smap1 Map.empty) \<alpha> F = \<alpha>"
-  using assms
-proof (induct)
-  case empty
-  then show ?case by auto
-next
-  case (insert x F)
-  hence "Finite_Set.fold (smap1 Map.empty) \<alpha> (insert x F) = 
-         smap1 Map.empty x (Finite_Set.fold (smap1 Map.empty) \<alpha> F)"
-    using cfi.fold_insert_idem by blast
-  also have "... = Finite_Set.fold (smap1 Map.empty) \<alpha> F" by auto
-  also have "... = \<alpha>" using insert(3) by blast
-  finally show ?case .
-qed
-
-subsection \<open>smap Theories\<close>
-
-lemma smap_rd [simp]:
-  "rd (smap \<beta> M) = rd \<beta> - dom M"
-proof -
-  have "finite (rd \<beta>)" by auto
-  thus ?thesis unfolding smap_def by auto
-qed
-
-lemma smap_wr [simp]:
-  "wr (smap \<beta> M) = wr \<beta>"
-proof -
-  have "finite (rd \<beta>)" by auto
-  thus ?thesis unfolding smap_def by auto
-qed
-
-lemma smap_barriers [simp]:
-  "barriers (smap \<beta> M) = barriers \<beta>"
-proof -
-  have "finite (rd \<beta>)" by auto
-  thus ?thesis unfolding smap_def by auto
-qed
-
-lemma smap_empty [simp]:
-  "smap \<beta> Map.empty = \<beta>"
-proof -
-  have "finite (rd \<beta>)" by auto
-  thus ?thesis using smap1_fold_empty unfolding smap_def by auto
-qed
-
-lemma smap_rep [simp]:
-  "smap1 M x (smap \<beta> M) = smap \<beta> M"
-proof (cases "x \<in> rd \<beta>")
-  case True
-  have "Finite_Set.fold (smap1 M) \<beta> (insert x (rd \<beta>)) =
-        smap1 M x (Finite_Set.fold (smap1 M) \<beta> (rd \<beta>))"
-    using cfi.fold_insert_idem by blast
-  moreover have "insert x (rd \<beta>) = rd \<beta>" using True by auto
-  ultimately show ?thesis unfolding smap_def by auto
-next
-  case False
-  thus ?thesis by simp
-qed
-
-subsection \<open>forall Theories\<close>
-
-lemma forall_rd [simp]:
-  "\<forall>\<alpha> \<in> forall V \<beta>. rd \<alpha> = rd \<beta> - V"
-  unfolding forall_def by auto
-
-lemma forall_wr [simp]:
-  "\<forall>\<alpha> \<in> forall V \<beta>. wr \<alpha> = wr \<beta>"
-  unfolding forall_def by auto
-
-lemma forall_barriers [simp]:
-  "\<forall>\<alpha> \<in> forall V \<beta>. barriers \<alpha> = barriers \<beta>"
-  unfolding forall_def by auto
-
-lemma forall_fence [simp]:
-  "\<forall>\<alpha> \<in> forall V \<beta>.  (\<alpha> \<noteq> full_fence) = (\<beta> \<noteq> full_fence)"
-proof -
-  have "\<forall>\<alpha>. barriers \<alpha> = (\<alpha> = full_fence)" by (intro allI, case_tac \<alpha>; auto)
-  thus ?thesis using forall_barriers by blast
-qed
-
-lemma forall_nil [simp]:
-  "forall {} \<alpha> = {\<alpha>}"
-  unfolding forall_def by auto
-
-lemma smap1_cong [intro]:
-  "M x = N x \<Longrightarrow> smap1 M x = smap1 N x"
-  unfolding smap1_def using domIff by fastforce
-
-lemma
-  "comp_fun_commute_on (rd \<alpha>) (smap1 (\<lambda>y. if x = y then None else M y))"
-  by (rule Finite_Set.comp_fun_commute_on.intro) auto
-
-lemma
-  "comp_fun_commute_on (rd \<alpha>) (smap1 (\<lambda>y. if x = y then None else M y))"
-  by (rule Finite_Set.comp_fun_commute_on.intro) auto
-  
-lemma forall_unfold:
-  shows "forall (insert x V) \<alpha> = {subst\<^sub>i \<alpha>' x (Val c) | c \<alpha>'. \<alpha>' \<in> forall V \<alpha>}" (is "?L = ?R")
-proof -
-  have "?L \<subseteq> ?R"
-  proof (clarsimp simp: forall_def, cases "x \<in> V")
-    fix M assume d: "dom (M :: ('b, 'c) SimAsm_State.var \<Rightarrow> 'a option) = insert x V" "x \<in> V"
-    hence "smap \<alpha> M = subst\<^sub>i (smap \<alpha> M) x (Val (the (M x)))" by simp
-    moreover have "dom M = V" using d by auto
-    ultimately show "\<exists>c \<alpha>'. smap \<alpha> M = subst\<^sub>i \<alpha>' x (Val c) \<and> (\<exists>M. \<alpha>' = smap \<alpha> M \<and> dom M = V)"
-      by blast
-  next
-    fix M assume d: "dom (M :: ('b, 'c) SimAsm_State.var \<Rightarrow> 'a option) = insert x V" "x \<notin> V"
-    let ?M = "\<lambda>y. if x = y then None else M y"
-    have "smap \<alpha> M = subst\<^sub>i (smap \<alpha> ?M) x (Val (the (M x)))"
-    proof -
-      have 
-        "comp_fun_commute_on (rd \<alpha>) (smap1 M)" 
-        "comp_fun_commute_on (rd \<alpha>) (smap1 (\<lambda>y. if x = y then None else M y))"
-        by standard auto
-      hence mx: "Finite_Set.fold (smap1 M) \<alpha> (rd \<alpha> - {x}) = Finite_Set.fold (smap1 ?M) \<alpha> (rd \<alpha> - {x})"
-        by (auto intro!: Finite_Set.fold_cong simp add: cfi.comp_fun_commute_axioms)
-      show ?thesis
-      proof (cases "x \<in> rd \<alpha>")
-        case True
-        hence [simp]: "insert x (rd \<alpha>) = rd \<alpha>" by auto
-        have fx: "Finite_Set.fold (smap1 M) \<alpha> (insert x (rd \<alpha>)) = 
-                  smap1 M x (Finite_Set.fold (smap1 M) \<alpha> (rd \<alpha> - {x}))"
-          by (rule cfi.fold_insert_remove) blast
-        have "Finite_Set.fold (smap1 ?M) \<alpha> (insert x (rd \<alpha>)) = 
-                  smap1 ?M x (Finite_Set.fold (smap1 ?M) \<alpha> (rd \<alpha> - {x}))"
-          by (rule cfi.fold_insert_remove) blast
-        also have "... = Finite_Set.fold (smap1 ?M) \<alpha> (rd \<alpha> - {x})" by auto
-        finally show ?thesis using fx mx unfolding smap_def apply simp
-          unfolding smap1_def using d(1) by (auto split: if_splits)
-      next
-        case False
-        hence [simp]: "rd \<alpha> - {x} = rd \<alpha>" by auto
-        have "x \<notin> rd (smap \<alpha> ?M)" using False by simp
-        then show ?thesis using mx unfolding smap_def by simp
-      qed
-    qed
-    moreover have "dom ?M = V" using d by (auto split: if_splits)
-    ultimately show "\<exists>c \<alpha>'. smap \<alpha> M = subst\<^sub>i \<alpha>' x (Val c) \<and> (\<exists>M. \<alpha>' = smap \<alpha> M \<and> dom M = V)"
-      by blast
-  qed
-
-  moreover have "?R \<subseteq> ?L"
-  proof (clarsimp simp: forall_def, cases "x \<in> V")
-    fix M c assume d: "V = dom (M :: ('b, 'c) SimAsm_State.var \<Rightarrow> 'a option)" "x \<in> V" 
-    have "dom M = insert x (dom M)" using d by auto
-    moreover have "subst\<^sub>i (smap \<alpha> M) x (Val c) = smap \<alpha> M" using d by simp
-    ultimately show "\<exists>Ma. subst\<^sub>i (smap \<alpha> M) x (Val c) = smap \<alpha> Ma \<and> dom Ma = insert x (dom M)"
-      by blast
-  next
-    fix M c assume d: "V = dom (M :: ('b, 'c) SimAsm_State.var \<Rightarrow> 'a option)" "x \<notin> V" 
-    let ?M = "\<lambda>y. if y = x then Some c else M y"
-    have "dom ?M = insert x (dom M)" using d by auto
-    moreover have "subst\<^sub>i (smap \<alpha> M) x (Val c) = smap \<alpha> ?M"
-    proof -
-      have 
-        "comp_fun_commute_on (rd \<alpha>) (smap1 M)" 
-        "comp_fun_commute_on (rd \<alpha>) (smap1 (\<lambda>y. if y = x then Some c else M y))"
-        by standard auto
-      hence mx: "Finite_Set.fold (smap1 M) \<alpha> (rd \<alpha> - {x}) = Finite_Set.fold (smap1 ?M) \<alpha> (rd \<alpha> - {x})"
-        by (auto intro!: Finite_Set.fold_cong simp add: cfi.comp_fun_commute_axioms)
-      show ?thesis
-      proof (cases "x \<in> rd \<alpha>")
-        case True
-        hence [simp]: "insert x (rd \<alpha>) = rd \<alpha>" by auto
-        have fx: "Finite_Set.fold (smap1 ?M) \<alpha> (insert x (rd \<alpha>)) = 
-                  smap1 ?M x (Finite_Set.fold (smap1 ?M) \<alpha> (rd \<alpha> - {x}))"
-          by (rule cfi.fold_insert_remove) blast
-        have "Finite_Set.fold (smap1 M) \<alpha> (insert x (rd \<alpha>)) = 
-                  smap1 M x (Finite_Set.fold (smap1 M) \<alpha> (rd \<alpha> - {x}))"
-          by (rule cfi.fold_insert_remove) blast
-        also have "... = Finite_Set.fold (smap1 M) \<alpha> (rd \<alpha> - {x})" using d by auto        
-        finally show ?thesis using fx mx unfolding smap_def apply simp
-          unfolding smap1_def using d(1) by (auto split: if_splits)
-      next
-        case False
-        hence [simp]: "rd \<alpha> - {x} = rd \<alpha>" by auto
-        have "x \<notin> rd (smap \<alpha> ?M)" using False by simp
-        then show ?thesis using mx unfolding smap_def by simp
-      qed
-    qed
-    ultimately show "\<exists>Ma. subst\<^sub>i (smap \<alpha> M) x (Val c) = smap \<alpha> Ma \<and> dom Ma = insert x (dom M)"
-      by blast
-  qed
-
-  ultimately show ?thesis by blast
-qed
-
-lemma forall_one [simp]:
-  "forall {x} \<alpha> = {subst\<^sub>i \<alpha> x (Val c) | c. True}"
-  unfolding forall_unfold[of x "{}" \<alpha>] by auto
-
-lemma forall_nop [simp]:
-  assumes "x \<notin> rd \<alpha>" 
-  shows "forall (insert x V) \<alpha> = forall V \<alpha>"
-  using assms forall_unfold by force
-
-lemma forallI [intro]:
-  "smap \<alpha> M \<in> forall (dom M) \<alpha>"
-  by (auto simp: forall_def)
-
-subsection \<open>Update lemmas\<close>
-
-definition upd                   (* use if f is a total fun: 'a \<Rightarrow> 'v *)
-  where "upd S f m \<equiv> m\<lparr>st := \<lambda>x. if x \<in> S then Some (f x) else st m x\<rparr>"
-
-definition upd_part       (* use if f is a partial fun: 'a \<Rightarrow> 'v option *)
-  where "upd_part S f m \<equiv> m\<lparr>st := \<lambda>x. if x \<in> S then (f x) else st m x\<rparr>"
-
-lemma upd_nil [simp]:
-  "upd {} f m = m"
-  by (auto simp: upd_def)
-
-
-lemma upd_insert' [simp]:
-  "upd (insert x V) f m = (upd V f m)(x :=\<^sub>s (f x))"
-  by (auto simp: upd_def st_upd_def intro!: state_rec.equality)
-
-(*
-lemma upd_rep [simp]:
-  "upd A (st (upd A f m\<^sub>1)) m\<^sub>2 = upd A f m\<^sub>2"
-  by (auto simp: upd_def intro!: state_rec.equality)
-*)
-
-lemma upd_rep [simp]:
-  "upd_part A (st (upd A f m\<^sub>1)) m\<^sub>2 = upd A f m\<^sub>2"
-  by (auto simp: upd_part_def upd_def intro!: state_rec.equality)
-
-lemma upd_rep' [simp]:
-  "upd A f (upd B f m) = upd (A \<union> B) f m"
-  by (auto simp: upd_def intro!: state_rec.equality)
-
-lemma upd_st [simp]:
-  "st (upd S f m) x = (if x \<in> S then Some (f x) else st m x)"
-  by (auto simp: upd_def)
-
-lemma upd_more [simp]:
-  "state_rec.more (upd V f m) = state_rec.more m"
-  by (auto simp: upd_def)
-
-lemma upd_cap [simp]:
-  "state_rec.cap (upd V f m) = state_rec.cap m"
-  by (auto simp: upd_def)
-
-lemma upd_init [simp]:
-  "state_rec.initState (upd V f m) = state_rec.initState m"
-  by (auto simp: upd_def)
-
-(* new: same updates on trees *)  
+subsection \<open>Update lemmas on trees\<close>
 
 definition updTree         (* assume total fun f : 'a \<longrightarrow> 'v *)
   where "updTree S f t \<equiv> 
@@ -785,7 +242,7 @@ proof -
   have a3:"tree_upd t (treeTop t\<lparr>st := ?f2\<rparr>) = tree_upd t ((treeTop (updTree V f t))(x :=\<^sub>s (f x)))" 
     using a2 by (auto simp: updTree_def st_upd_def intro!: state_rec.equality) 
   have a4:"tree_upd t (treeTop t\<lparr>st := ?f1\<rparr>) = updTree (insert x V) f t"
-    by (auto simp: updTree_def st_upd_def upd_def intro!: state_rec.equality)   
+    by (auto simp: updTree_def st_upd_def  intro!: state_rec.equality)   
   have a5:"updTree (insert x V) f t = tree_upd t ((treeTop (updTree V f t))(x :=\<^sub>s (f x)))"
     using a3 a4 a2 by simp
   thus ?thesis by simp
@@ -882,36 +339,6 @@ lemma based_updTree_single:
   by fastforce
 
 
-(*
-thm state_rec.equality
-
-state_rec.equality:
- equality: st ?r = st ?r' 
-       \<Longrightarrow> cap ?r = cap ?r' 
-       \<Longrightarrow> initState ?r = initState ?r'
-       \<Longrightarrow> more ?r = more ?r'                    \<Longrightarrow> ?r = ?r'
-*)
-
-
-(* do we need this version?
-lemma updTree_insert' [simp]:
-  "updTree (insert x V) f t = tr_up (updTree V f t) x (f x)"
-(*  apply (auto simp: updTree_def tr_upd_def intro!:state_rec.equality) *)
-proof -
-  let ?f1 = "\<lambda>xa. if xa = x \<or> xa \<in> V then Some (f xa) else st (treeTop t) xa"
-  let ?f2 = "\<lambda>x. if x \<in> V then Some (f x) else st (treeTop t) x"
-  have a0: "tree_upd t (treeTop t\<lparr>st := ?f1\<rparr>) = tr_upd (tree_upd t (treeTop t\<lparr>st := ?f2\<rparr>)) x (f x)" sorry
-  then show ?thesis using updTree_def 
-*)
-
-(* if \<Gamma> is in aux then this will include equality of \<Gamma> mapping *)
-lemma st_upd_eq [intro]:
-  "state_rec.more m = state_rec.more m' \<Longrightarrow> 
-              state_rec.cap m = state_rec.cap m' \<Longrightarrow>
-                 initState m = initState m' \<Longrightarrow>
-                    \<forall>x. x \<noteq> y \<longrightarrow> st m x = st m' x \<Longrightarrow> m(y :=\<^sub>s e) = m'(y :=\<^sub>s e)"
-  by (auto simp: upd_def st_upd_def intro!: state_rec.equality)
-
 lemma help_rep:
   assumes "x \<in> A \<Longrightarrow> (st (upd_part A f m) x) = (f x)"
   shows "(\<lambda>x. if x \<in> A then (st (upd_part A f m) x) else (st (treeTop t) x)) =
@@ -975,48 +402,26 @@ lemma updTreePart_init [simp]:
   by (auto simp: updTree_part_def)
 
 
-lemma [simp]:
-  "rg (upd_part V f m) x = (if Reg x \<in> V then f (Reg x) else rg m x)"
-  unfolding rg_def upd_part_def
-  by simp
-
-lemma [simp]:
-  "rg (m(aux: f)) = rg m"
-  unfolding rg_def aux_upd_def by simp
-
-
-
-lemma eq_comm:
-  "(a \<Longrightarrow> (b = c)) \<Longrightarrow> (a \<Longrightarrow> (c = b))" by blast
-
-
-thm state_rec.equality
-
 lemma treeBase_equality:
   "s\<^sub>1 = s\<^sub>2 \<Longrightarrow> (Base s\<^sub>1) = (Base s\<^sub>2)" by auto
 
 lemma treeBranch_equality:
   "t\<^sub>1 = t\<^sub>1' \<Longrightarrow> t\<^sub>2 = t\<^sub>2' \<Longrightarrow> Branch t\<^sub>1 t\<^sub>2 = Branch t\<^sub>1' t\<^sub>2'" by auto 
 
-
-(* lemma beh_substi [simp]:
-  "beh\<^sub>i (subst\<^sub>i \<alpha> x e) = {(m\<^sub>1,upd (wr \<alpha>) (st m) m\<^sub>1) |m m\<^sub>1. (m\<^sub>1(x :=\<^sub>s ev\<^sub>E m\<^sub>1 e),m) \<in> beh\<^sub>i \<alpha>}"
- *)
-
 (* this lemma needs to be split up into different cases (above) as it does not hold for leak instr *)
 
 lemma beh_subst\<^sub>i_nonleak:
   assumes "\<And>y z. \<alpha> \<noteq> leak y z"
   shows   "beh\<^sub>i (subst\<^sub>i \<alpha> x e) = 
-              {(t, updTree (wr \<alpha>) (lookupSome t') t) |t t'. (t(x :=\<^sub>t ev\<^sub>E t e), t') \<in> beh\<^sub>i \<alpha>}"
+              {(t, updTree (wr \<alpha>) (lookupSome t') t) |t t'. (t(x :=\<^sub>t tr_ev\<^sub>E t e), t') \<in> beh\<^sub>i \<alpha>}"
 proof (cases \<alpha>)
   case (assign x11 x12)
   then show ?thesis 
-    by auto (simp_all add: st_upd_def tr_upd_def)
+    sorry (*by auto (simp_all add: st_upd_def tr_upd_def)*)
 next
   case (cmp x2)
   then show ?thesis
-    using ev_subst\<^sub>B ev_subst\<^sub>B' by auto
+    using tr_ev_subst\<^sub>B tr_ev_subst\<^sub>B' sorry
 next
   case full_fence
   then show ?thesis by auto
@@ -1032,25 +437,25 @@ qed
 lemma beh_subst\<^sub>i_assign [simp]:
   assumes "\<alpha> = assign y z"
   shows   "beh\<^sub>i (subst\<^sub>i \<alpha> x e) = 
-              {(t, updTree (wr \<alpha>) (lookupSome t') t) |t t'. (t(x :=\<^sub>t ev\<^sub>E t e), t') \<in> beh\<^sub>i \<alpha>}"
+              {(t, updTree (wr \<alpha>) (lookupSome t') t) |t t'. (t(x :=\<^sub>t tr_ev\<^sub>E t e), t') \<in> beh\<^sub>i \<alpha>}"
   by (rule beh_subst\<^sub>i_nonleak) (simp add: assms)
 
 lemma beh_subst\<^sub>i_cmp [simp]:
   assumes "\<alpha> = cmp b"
   shows   "beh\<^sub>i (subst\<^sub>i \<alpha> x e) = 
-              {(t, updTree (wr \<alpha>) (lookupSome t') t) |t t'. (t(x :=\<^sub>t ev\<^sub>E t e), t') \<in> beh\<^sub>i \<alpha>}"
+              {(t, updTree (wr \<alpha>) (lookupSome t') t) |t t'. (t(x :=\<^sub>t tr_ev\<^sub>E t e), t') \<in> beh\<^sub>i \<alpha>}"
   by (rule beh_subst\<^sub>i_nonleak) (simp add: assms)
 
 lemma beh_subst\<^sub>i_fence [simp]:
   assumes "\<alpha> = full_fence"
   shows   "beh\<^sub>i (subst\<^sub>i \<alpha> x e) = 
-              {(t, updTree (wr \<alpha>) (lookupSome t') t) |t t'. (t(x :=\<^sub>t ev\<^sub>E t e), t') \<in> beh\<^sub>i \<alpha>}"
+              {(t, updTree (wr \<alpha>) (lookupSome t') t) |t t'. (t(x :=\<^sub>t tr_ev\<^sub>E t e), t') \<in> beh\<^sub>i \<alpha>}"
   by (rule beh_subst\<^sub>i_nonleak) (simp add: assms)  
 
 lemma beh_subst\<^sub>i_nop [simp]:
   assumes "\<alpha> = nop"
   shows   "beh\<^sub>i (subst\<^sub>i \<alpha> x e) = 
-              {(t, updTree (wr \<alpha>) (lookupSome t') t) |t t'. (t(x :=\<^sub>t ev\<^sub>E t e), t') \<in> beh\<^sub>i \<alpha>}"
+              {(t, updTree (wr \<alpha>) (lookupSome t') t) |t t'. (t(x :=\<^sub>t tr_ev\<^sub>E t e), t') \<in> beh\<^sub>i \<alpha>}"
   by (rule beh_subst\<^sub>i_nonleak) (simp add: assms) 
 (*---*)
 
@@ -1058,21 +463,21 @@ lemma beh_subst\<^sub>i_nop [simp]:
 lemma beh_subst\<^sub>i_leak [simp]:
   assumes "\<alpha> = leak y z"
   shows   "beh\<^sub>i (subst\<^sub>i \<alpha> x e) =
-              {(t, updTree_base (wr \<alpha>) (lookupSome t') t) |t t'. (t(x :=\<^sub>t ev\<^sub>E t e), t') \<in> beh\<^sub>i \<alpha>}"
+              {(t, updTree_base (wr \<alpha>) (lookupSome t') t) |t t'. (t(x :=\<^sub>t tr_ev\<^sub>E t e), t') \<in> beh\<^sub>i \<alpha>}"
   using assms
   apply auto
-   apply (case_tac "lookup (a(x :=\<^sub>t ev\<^sub>E a e, y :=\<^sub>b ev\<^sub>E (a(x :=\<^sub>t ev\<^sub>E a e)) z)) y")
+   apply (case_tac "lookup (a(x :=\<^sub>t tr_ev\<^sub>E a e, y :=\<^sub>b tr_ev\<^sub>E (a(x :=\<^sub>t tr_ev\<^sub>E a e)) z)) y")
     apply auto
     apply (metis lookup_tr_base_upd option.simps(3))
    defer
-   apply (case_tac "lookup (t(x :=\<^sub>t ev\<^sub>E t e, y :=\<^sub>b ev\<^sub>E (t(x :=\<^sub>t ev\<^sub>E t e)) z)) y")
+   apply (case_tac "lookup (t(x :=\<^sub>t tr_ev\<^sub>E t e, y :=\<^sub>b tr_ev\<^sub>E (t(x :=\<^sub>t tr_ev\<^sub>E t e)) z)) y")
     apply auto
     apply (metis lookup_tr_base_upd option.distinct(1))
 proof goal_cases
   case (1 t a)
   hence "based t y" "x \<noteq> y" sorry (* are these assumptions required ? ! if so, where? *)
-  hence a: "ev\<^sub>E (t(x :=\<^sub>t ev\<^sub>E t e)) z = a" using 1 based_tr_upd 
-    sorry  then show c: "t(y :=\<^sub>b a) = t(y :=\<^sub>b ev\<^sub>E (t(x :=\<^sub>t ev\<^sub>E t e)) z)" using 1 by simp
+  hence a: "tr_ev\<^sub>E (t(x :=\<^sub>t tr_ev\<^sub>E t e)) z = a" using 1 based_tr_upd  sorry  
+  then have c: "t(y :=\<^sub>b a) = t(y :=\<^sub>b tr_ev\<^sub>E (t(x :=\<^sub>t tr_ev\<^sub>E t e)) z)" using 1 sorry
   (* there is another possibility. 
   we do not strictly need the fact (a), we just need to show the ?case. 
   this could be done by arguing in this way: 
@@ -1080,166 +485,12 @@ proof goal_cases
     - if y is not based in t, then (c) could be argued since y's base update will be hidden in 
       both states, and so they are "visually equivalent" at that time.
   *)
+  then show ?case sorry 
 next
   case (2 t a)
   show ?case using 2 sorry (* identical argument to 1 *)
 qed
-(*
-proof -
-  have a0:"beh\<^sub>i (subst\<^sub>i \<alpha> x e) = beh\<^sub>i (leak y (subst\<^sub>E z x e))" using assms by simp
-  then have a1:"... = {(t,t'). t' = tree_base_upd t ((base t) (y :=\<^sub>s (ev\<^sub>E (t) (subst\<^sub>E z x e))))}" by simp
-  then have a2:"... = {(t,t'). 
-       t' = updTree_base (wr \<alpha>) (lookupSome(tree_base_upd t ((base t) (y :=\<^sub>s (ev\<^sub>E (t) (subst\<^sub>E z x e)))))) t}"
-    using assms 
-    apply auto sorry
-  then have a3:"... = {(t,t'). t' = 
-         updTree_base (wr \<alpha>) (lookupSome(tree_base_upd t ((base t)(y :=\<^sub>s (ev\<^sub>E (t (x :=\<^sub>t (ev\<^sub>E t e))) z))))) t}"
-    using ev_subst\<^sub>E by auto
-  then have a4:"... = {(t,t')| t t' t''. t'' = t(x :=\<^sub>t (ev\<^sub>E t e)) \<and>
-                    t'= updTree_base (wr \<alpha>) (lookupSome(tree_base_upd t ((base t)(y :=\<^sub>s (ev\<^sub>E t'' z))))) t}"
-    by auto
-    then show ?thesis using assms a1 a2 a3 sorry
-  qed
-*)
-
-lemma [simp]:
-  "st (m(x :=\<^sub>s e)) = (st m)(x := Some e)"
-  by (auto simp: st_upd_def)
-
-lemma [simp]:
-  "Base (st (m(x :=\<^sub>s e))) = Base ((st m)(x := Some e))"
-  by (auto simp: st_upd_def)
 
 
 
-(*todo: smap1 lemmas only needed for static analysis part (to compute reorderable pairs?)
-        leave for now  *)
-
-(* 
-lemma beh_smap1 [simp]:
-  "beh\<^sub>i (smap1 M x \<alpha>) = {(m\<^sub>1,upd (wr \<alpha>) (st m) m\<^sub>1) |m m\<^sub>1.(upd ({x} \<inter> dom M) (the o M) m\<^sub>1,m) \<in> beh\<^sub>i \<alpha>}"
-by (cases \<alpha> ; auto simp: smap1_def) 
-*)
-
-(*
-lemma "{(t,t')| t t'. t=t'} = {(t,t)|t. 1=1}" by simp 
-
-lemma stUpd_trUpd:
-  assumes "(M x) \<noteq> None"
-  shows "(top t)\<lparr>st := \<lambda>y. if y \<in> {x} then (M y) else st (top t) y\<rparr> = top (t (x :=\<^sub>t the (M x)))"
-  using  assms tr_upd_def 
-proof -
-  have a0:"top t\<lparr>st := \<lambda>y. if y \<in> {x} then M y else st (top t) y\<rparr> = 
-              top t\<lparr>st := ((st (top t)) (x := (M x)))\<rparr>"
-    apply (rule equality) apply simp by auto 
-  then have a1:"top t\<lparr>st := ((st (top t)) (x := (M x)))\<rparr> =
-                  top (t(x :=\<^sub>t the (M x)))" using assms tr_upd_def sorry
-  then show ?thesis  using a0 a1 by simp
-qed
-
-
-lemma ev_updTreePart:
-  assumes "(M x) \<noteq> None"
-  shows   "ev\<^sub>B (updTree_part ({x} \<inter> dom M) M t) b =
-                     ev\<^sub>B t (if (x \<in> dom M) then (subst\<^sub>B b x (Val(the (M x)))) else b)"
-proof -
-  have a0:"({x} \<inter> dom M) = (if (x \<in> (dom M)) then {x} else {})" by simp
-  have a1:"({x} \<inter> dom M) \<noteq> {} \<equiv> x \<in> dom M" by simp
-  have a2:"updTree_part ({x} \<inter> dom M) M t = 
-        tree_upd t ((top t)\<lparr>st := \<lambda>y. if y \<in> ({x} \<inter> (dom M)) then (M y) else st (top t) y\<rparr>)" 
-    using updTree_part_def by blast
-  have c1:"updTree_part {} M t = t" using  updTreePart_nil by simp
-  have c2:"x \<in> dom M \<Longrightarrow> 
-          updTree_part ({x} \<inter> dom M) M t =  updTree_part {x} M t" using a0 by presburger 
-  then have c3:"... = tree_upd t ((top t)\<lparr>st := \<lambda>y. if y \<in> {x} then (M y) else st (top t) y\<rparr>)"
-    using updTree_part_def by blast
-  hence d1:"updTree_part ({x} \<inter> dom M) M t = 
-            (if x \<in> dom M then tree_upd t ((top t)\<lparr>st := \<lambda>y. if y \<in> {x} then (M y) else st (top t) y\<rparr>)
-                         else t)" using a0 a1 c3 a2 by simp
-  then have d2:"... = (if x \<in> dom M then tree_upd t (top (t (x :=\<^sub>t the (M x))))
-                         else t)" using stUpd_trUpd assms sorry
-  then show ?thesis using d1 d2 
-    by (smt (verit, ccfv_threshold) ev\<^sub>E.simps(2) ev_subst\<^sub>B' top_treeUpd tr_upd_def)
-qed
-
-lemma beh_smap1 [simp]:
-  "beh\<^sub>i (smap1 M x \<alpha>) = {(t,updTree (wr \<alpha>) (lookupSome t') t) |t t'.
-                           (updTree_part ({x} \<inter> dom M) (M) t,t') \<in> beh\<^sub>i \<alpha>}"
-(*  apply (cases \<alpha> ; auto simp: smap1_def updTree_def updTree_part_def) *)
-proof (cases \<alpha>)
-  case (assign x11 x12)
-  then show ?thesis sorry
-next
-  case (cmp b)
-  then show ?thesis 
-  proof -
-    have a0:"smap1 M x (cmp b) = (if x \<in> dom M then subst\<^sub>i (cmp b) x (Val (the (M x))) else (cmp b))"
-       using smap1_def cmp by blast
-     then have a1:"beh\<^sub>i (smap1 M x (cmp b)) = 
-         {(t,t'). t=t' \<and> ev\<^sub>B t (if (x \<in> dom M) then (subst\<^sub>B b x (Val(the (M x)))) else b)}" 
-      using smap1_def beh\<^sub>i.simps(2) subst\<^sub>i.simps(2) cmp by force
-    then have a2:"... = {(t,t)| t . ev\<^sub>B t (if (x \<in> dom M) then (subst\<^sub>B b x (Val(the (M x)))) else b)}"
-      using a1 by blast
-    have b0:"wr(cmp b) = {}" by simp
-    have b1:"\<forall> t t'. updTree (wr (cmp b)) (lookupSome t') t = t" using updTree_def b0 by simp
-    then have b2:"{(t,updTree(wr(cmp b))(lookupSome t') t)|t t'.
-                                  (updTree_part ({x} \<inter> dom M) M t, t') \<in> beh\<^sub>i (cmp b)} = 
-                    {(t,t)| t t'. (updTree_part ({x} \<inter> dom M) M t, t') \<in> beh\<^sub>i (cmp b)}" 
-      using b1 by simp
-    then have b3:"... = {(t,t)| t. ev\<^sub>B (updTree_part ({x} \<inter> dom M) M t) b}" using b2 beh\<^sub>i.simps(2) 
-         by simp
-    then have b4:"... = {(t,t)| t . ev\<^sub>B t (if (x \<in> dom M) then (subst\<^sub>B b x (Val(the (M x)))) else b)}"
-      using ev_updTreePart sorry
-    then show ?thesis using a0 a1 a2 b1 b2 b3 cmp by (smt (verit, del_insts) Collect_cong)
-  qed
-qed auto
-*)
-
-(*
-
-lemma beh_fold_smap1:
-  assumes "finite F" 
-  shows "beh\<^sub>i (Finite_Set.fold (smap1 M) \<alpha> F) = {(m\<^sub>1, upd_part (wr \<alpha>) (st m) m\<^sub>1) |m m\<^sub>1. (upd (F \<inter> dom M) (the \<circ> M) m\<^sub>1, m) \<in> beh\<^sub>i \<alpha>}"
-  using assms
-proof (induct)
-  case empty
-  then show ?case apply (cases \<alpha> ; auto) sorry
-next
-  case (insert x F)
-  hence f: "Finite_Set.fold (smap1 M) \<alpha> (insert x F) = 
-         smap1 M x (Finite_Set.fold (smap1 M) \<alpha> F)"
-    using cfi.fold_insert_idem by blast
-
-  show ?case using insert(1)
-    unfolding f beh_smap1 insert(3)
-    apply auto unfolding o_def 
-    apply (intro exI conjI)
-    apply blast
-    sorry
-(*  
-  apply (metis Int_Un_distrib2 Un_insert_right inf_bot_right sup_inf_absorb)
-    apply (intro exI conjI)
-    prefer 2
-    apply blast
-    apply simp
-    apply (metis Int_Un_distrib2 Un_insert_right inf_bot_right sup_inf_absorb)
-    done
-*)
-qed
-
-
-lemma beh_smap [simp]:
-  "beh\<^sub>i (smap \<alpha> M) = {(m\<^sub>1,upd_part (wr \<alpha>) (st m) m\<^sub>1) | m m\<^sub>1. (upd (dom M) (the o M) m\<^sub>1,m) \<in> beh\<^sub>i \<alpha>}"
-proof -
-  have "finite (rd \<alpha>)" by auto
-  hence "beh\<^sub>i (Finite_Set.fold (smap1 M) \<alpha> (rd \<alpha>)) = 
-          {(m\<^sub>1, upd_part (wr \<alpha>) (st m) m\<^sub>1) |m m\<^sub>1. (upd ((rd \<alpha>) \<inter> dom M) (the \<circ> M) m\<^sub>1, m) \<in> beh\<^sub>i \<alpha>}"
-    using beh_fold_smap1 by blast
-
-  also have "... = {(m\<^sub>1, upd_part (wr \<alpha>) (st m) m\<^sub>1) |m m\<^sub>1. (upd (dom M) (the \<circ> M) m\<^sub>1, m) \<in> beh\<^sub>i \<alpha>}"
-    apply (cases \<alpha>; auto)
- sorry
-  finally show ?thesis unfolding smap_def .
-qed
-*)
 end
