SimAsm/Var_map.thy
@@ -3,11 +3,17 @@ theory Var_map
 
 begin
 
+
 (* variable: either a register or a global, where registers equal local vars *)
 datatype 'r Reg = reg 'r | tmp 'r
 datatype ('g,'r) var = Reg 'r | Glb 'g
 
-print_theorems
+(*
+locale expression = state 
+
+context expression
+begin
+*)
 
 definition glb' :: "(('g,'r) var \<Rightarrow> 'v) \<Rightarrow> ('g \<Rightarrow> 'v)"
   where "glb' m \<equiv> \<lambda>v. m (Glb v)"
@@ -37,11 +43,11 @@ datatype ('v,'g,'r) exp =
 
 text \<open>Evaluate an expression given a state\<close>
 
-fun ev\<^sub>E' :: "(('g,'r) var \<Rightarrow> 'v) \<Rightarrow> ('v,'g,'r) exp \<Rightarrow> 'v"
+fun ev\<^sub>E :: "(('g,'r) var \<Rightarrow> 'v) \<Rightarrow> ('v,'g,'r) exp \<Rightarrow> 'v"
   where 
-    "ev\<^sub>E' m (Var r) =  m r" |
-    "ev\<^sub>E' _ (Val v) = v" |
-    "ev\<^sub>E' m (Exp f rs) = f (map (ev\<^sub>E' m) rs)"  (* eg, Exp(+ a1 a2 a3) = (ev a1) + (ev a2) + (ev a3) *)
+    "ev\<^sub>E m (Var r) =  m r" |
+    "ev\<^sub>E _ (Val v) = v" |
+    "ev\<^sub>E m (Exp f rs) = f (map (ev\<^sub>E m) rs)"  (* eg, Exp(+ a1 a2 a3) = (ev a1) + (ev a2) + (ev a3) *)
 
 text \<open>The syntactic dependencies of an expression\<close>
 fun deps\<^sub>E :: "('v,'g,'r) exp \<Rightarrow> ('g,'r) var set"
@@ -63,10 +69,10 @@ datatype ('v,'g,'r) bexp =
   Exp\<^sub>B "'v list \<Rightarrow> bool" "('v,'g,'r) exp list"
 
 text \<open>Evaluate an expression given a state \<close>
-fun ev\<^sub>B' :: "(('g,'r) var\<Rightarrow> 'v) \<Rightarrow> ('v,'g,'r) bexp \<Rightarrow> bool"
+fun ev\<^sub>B :: "(('g,'r) var\<Rightarrow> 'v) \<Rightarrow> ('v,'g,'r) bexp \<Rightarrow> bool"
   where 
-    "ev\<^sub>B' m (Neg e) = (\<not> (ev\<^sub>B' m e))" |
-    "ev\<^sub>B' m (Exp\<^sub>B f rs) = f (map (ev\<^sub>E' m) rs)"
+    "ev\<^sub>B m (Neg e) = (\<not> (ev\<^sub>B m e))" |
+    "ev\<^sub>B m (Exp\<^sub>B f rs) = f (map (ev\<^sub>E m) rs)"
 
 text \<open>The syntactic dependencies of an expression\<close>
 fun deps\<^sub>B :: "('v,'g,'r) bexp \<Rightarrow> ('g,'r) var set"
@@ -167,19 +173,19 @@ lemma [simp]:
 
 
 lemma ev_subst\<^sub>E' [simp]:
-  "ev\<^sub>E' m (subst\<^sub>E e r f) = ev\<^sub>E' (m (r := (ev\<^sub>E' m f))) e"
+  "ev\<^sub>E m (subst\<^sub>E e r f) = ev\<^sub>E (m (r := (ev\<^sub>E m f))) e"
 proof (induct e)
   case (Exp fn rs)
-  hence [simp]: "map (ev\<^sub>E' m \<circ> (\<lambda>x. subst\<^sub>E x r f)) rs = map (ev\<^sub>E' (m(r := ev\<^sub>E' m f))) rs" 
+  hence [simp]: "map (ev\<^sub>E m \<circ> (\<lambda>x. subst\<^sub>E x r f)) rs = map (ev\<^sub>E (m(r := ev\<^sub>E m f))) rs" 
     using fun_upd_def apply auto using Exp by presburger
   then show ?case by (simp add: fun_upd_def)
 qed auto
 
 lemma ev_subst\<^sub>B [simp]:
-  "ev\<^sub>B' m (subst\<^sub>B b r e) = ev\<^sub>B' (m(r := (ev\<^sub>E' m e))) b"
+  "ev\<^sub>B m (subst\<^sub>B b r e) = ev\<^sub>B (m(r := (ev\<^sub>E m e))) b"
 proof (induct b)
   case (Exp\<^sub>B fn rs)
-  have [simp]: "map (ev\<^sub>E' m \<circ> (\<lambda>x. subst\<^sub>E x r e)) rs = map (ev\<^sub>E' (m(r := ev\<^sub>E' m e))) rs"
+  have [simp]: "map (ev\<^sub>E m \<circ> (\<lambda>x. subst\<^sub>E x r e)) rs = map (ev\<^sub>E (m(r := ev\<^sub>E m e))) rs"
     by (auto simp: fun_upd_def)     
   then show ?case by (simp add: fun_upd_def)
 qed simp
@@ -193,21 +199,21 @@ proof (induct e)
 qed auto
 
 lemma ev_nop\<^sub>E' [simp]:
-  "r \<notin> deps\<^sub>E e \<Longrightarrow> ev\<^sub>E' (m(r := f)) e = ev\<^sub>E' m e"
+  "r \<notin> deps\<^sub>E e \<Longrightarrow> ev\<^sub>E (m(r := f)) e = ev\<^sub>E m e"
 proof (induct e)
   case (Exp fn rs)
-  hence [simp]: "map (ev\<^sub>E' (m(r := f))) rs = map (ev\<^sub>E' m) rs" 
+  hence [simp]: "map (ev\<^sub>E (m(r := f))) rs = map (ev\<^sub>E m) rs" 
     using fun_upd_def apply auto using Exp by blast
-  then show ?case by (metis ev\<^sub>E'.simps(3))
+  then show ?case by (metis ev\<^sub>E.simps(3))
 qed auto
 
 lemma ev_nop\<^sub>B [simp]:
-  "r \<notin> deps\<^sub>B b \<Longrightarrow> ev\<^sub>B' (m(r := f)) b = ev\<^sub>B' m b"
+  "r \<notin> deps\<^sub>B b \<Longrightarrow> ev\<^sub>B (m(r := f)) b = ev\<^sub>B m b"
 proof (induct b)
   case (Exp\<^sub>B fn rs)
-  hence [simp]: "map (ev\<^sub>E' (m(r := f))) rs = map (ev\<^sub>E' m) rs"
-    using ev_nop\<^sub>E[of r _ m f] by (auto simp: fun_upd_def) 
-  then show ?case by (metis ev\<^sub>B'.simps(2))
+  hence [simp]: "map (ev\<^sub>E (m(r := f))) rs = map (ev\<^sub>E m) rs"
+    using ev_nop\<^sub>E'[of r _ m f] by (auto simp: fun_upd_def) 
+  then show ?case by (metis ev\<^sub>B.simps(2))
 qed simp
 
 lemma subst_nop\<^sub>B [simp]:
@@ -229,10 +235,10 @@ lemma deps_subst\<^sub>B [simp]:
 
                                     
 lemma deps_ev\<^sub>E [intro]:
-  "\<forall>x \<in> deps\<^sub>E e. m x = m' x \<Longrightarrow> ev\<^sub>E' m e = ev\<^sub>E' m' e"
+  "\<forall>x \<in> deps\<^sub>E e. m x = m' x \<Longrightarrow> ev\<^sub>E m e = ev\<^sub>E m' e"
 proof (induct e)
   case (Exp fn rs)
-  hence [simp]: "map (ev\<^sub>E' m) rs = map (ev\<^sub>E' m') rs" by (induct rs) auto
+  hence [simp]: "map (ev\<^sub>E m) rs = map (ev\<^sub>E m') rs" by (induct rs) auto
   show ?case by simp
 qed auto
 
@@ -250,14 +256,413 @@ lemma finite_deps\<^sub>E [intro]:
   by (induct e) auto
 
 
-lemma local_ev\<^sub>E' [intro]:
-  "deps\<^sub>E e \<subseteq> locals \<Longrightarrow> rg' m = rg' m' \<Longrightarrow> ev\<^sub>E' m e = ev\<^sub>E' m' e"
+lemma local_ev\<^sub>E [intro]:
+  "deps\<^sub>E e \<subseteq> locals \<Longrightarrow> rg' m = rg' m' \<Longrightarrow> ev\<^sub>E m e = ev\<^sub>E m' e"
   apply (intro deps_ev\<^sub>E ballI, case_tac x) 
   using rg'_def apply force
   using rg'_def by force
 
+subsection \<open>Operations\<close>
 
+lemma subst_wr [simp]:
+  "wr (subst\<^sub>i \<alpha> x e) = wr \<alpha>"
+  by (cases \<alpha>; auto)
+
+lemma subst_rd [simp]:
+  "rd (subst\<^sub>i \<alpha> x e) = rd \<alpha> - {x} \<union> (if x \<in> rd \<alpha> then deps\<^sub>E e else {})"
+  by (cases \<alpha>; auto)
+
+lemma subst_barriers [simp]:
+  "barriers (subst\<^sub>i \<alpha> x e) = barriers \<alpha>"
+  by (cases \<alpha>; auto)
+
+lemma subst_not_fence [simp]:
+  "(subst\<^sub>i \<alpha> x e \<noteq> full_fence) = (\<alpha> \<noteq> full_fence)"
+  by (cases \<alpha>; auto)
+
+lemma subst_nop [simp]:
+  "x \<notin> rd \<beta> \<Longrightarrow> subst\<^sub>i \<beta> x e = \<beta>"
+  unfolding smap1_def by (cases \<beta>) (auto split: if_splits)
+
+lemma finite_rd [intro]:
+  "finite (rd \<alpha>)"  
+proof  (cases \<alpha>)
+  case (cmp x2)
+  then show ?thesis sorry
+qed auto  
+
+abbreviation ncmp
+  where "ncmp b \<equiv> cmp (Neg b)"
+
+
+subsection \<open>smap1 Theories\<close>
+
+lemma smap1_flip [simp]:
+  "smap1 V y (smap1 V x \<alpha>) = smap1 V x (smap1 V y \<alpha>)" sorry
+(*  by (cases \<alpha>; cases "x = y"; auto simp: smap1_def)*)
+
+lemma smap1_rep [simp]:
+  "smap1 V x (smap1 V x \<alpha>) = smap1 V x \<alpha>"
+  by (cases \<alpha>; auto simp: smap1_def)
+
+interpretation cfi: comp_fun_idem "smap1 V"  by standard auto
+
+lemma smap1_rd [simp]:
+  "rd (smap1 M x \<beta>) = rd \<beta> - ({x} \<inter> dom M)"
+  unfolding smap1_def by (auto split: if_splits)
+
+lemma smap1_wr [simp]:
+  "wr (smap1 M x \<beta>) = wr \<beta>"
+  unfolding smap1_def by (auto split: if_splits)
+
+lemma smap1_barriers [simp]:
+  "barriers (smap1 M x \<beta>) = barriers \<beta>"
+  unfolding smap1_def by (auto split: if_splits)
+
+lemma smap1_nop [simp]:
+  "x \<notin> rd \<beta> \<Longrightarrow> smap1 M x \<beta> = \<beta>"
+  unfolding smap1_def by (auto split: if_splits)
+
+lemma smap1_nop2 [simp]:
+  "M x = None \<Longrightarrow> smap1 M x \<beta> = \<beta>"
+  unfolding smap1_def by (auto split: if_splits)
+
+lemma smap1_empty [simp]:
+  "smap1 Map.empty x \<beta> = \<beta>"
+  unfolding smap1_def by (auto split: if_splits)
+
+lemma smap1_fold_rd [simp]:
+  assumes "finite F"
+  shows "rd (Finite_Set.fold (smap1 M) \<beta> F) = rd \<beta> - (dom M \<inter> F)"
+  using assms
+proof (induct)
+  case empty
+  then show ?case by auto
+next
+  case (insert x F)
+  hence "Finite_Set.fold (smap1 M) \<beta> (insert x F) = smap1 M x (Finite_Set.fold (smap1 M) \<beta> F)"
+    using cfi.fold_insert_idem by blast
+  then show ?case by (auto simp: insert(3))
+qed
+
+lemma smap1_fold_wr [simp]:
+  assumes "finite F"
+  shows "wr (Finite_Set.fold (smap1 M) \<beta> F) = wr \<beta>"
+  using assms
+proof (induct)
+  case empty
+  then show ?case by auto
+next
+  case (insert x F)
+  hence "Finite_Set.fold (smap1 M) \<beta> (insert x F) = smap1 M x (Finite_Set.fold (smap1 M) \<beta> F)"
+    using cfi.fold_insert_idem by blast
+  then show ?case by (auto simp: insert(3))
+qed
+
+lemma smap1_fold_barriers [simp]:
+  assumes "finite F"
+  shows "barriers (Finite_Set.fold (smap1 M) \<beta> F) = barriers \<beta>"
+  using assms
+proof (induct)
+  case empty
+  then show ?case by auto
+next
+  case (insert x F)
+  hence "Finite_Set.fold (smap1 M) \<beta> (insert x F) = smap1 M x (Finite_Set.fold (smap1 M) \<beta> F)"
+    using cfi.fold_insert_idem by blast
+  then show ?case by (auto simp: insert(3))
+qed
+
+lemma smap1_fold_empty:
+  assumes "finite F"
+  shows "Finite_Set.fold (smap1 Map.empty) \<alpha> F = \<alpha>"
+  using assms
+proof (induct)
+  case empty
+  then show ?case by auto
+next
+  case (insert x F)
+  hence "Finite_Set.fold (smap1 Map.empty) \<alpha> (insert x F) = 
+         smap1 Map.empty x (Finite_Set.fold (smap1 Map.empty) \<alpha> F)"
+    using cfi.fold_insert_idem by blast
+  also have "... = Finite_Set.fold (smap1 Map.empty) \<alpha> F" by auto
+  also have "... = \<alpha>" using insert(3) by blast
+  finally show ?case .
+qed
+
+subsection \<open>smap Theories\<close>
+
+lemma smap_rd [simp]:
+  "rd (smap \<beta> M) = rd \<beta> - dom M"
+proof -
+  have "finite (rd \<beta>)" by auto
+  thus ?thesis unfolding smap_def by auto
+qed
+
+lemma smap_wr [simp]:
+  "wr (smap \<beta> M) = wr \<beta>"
+proof -
+  have "finite (rd \<beta>)" by auto
+  thus ?thesis unfolding smap_def by auto
+qed
+
+lemma smap_barriers [simp]:
+  "barriers (smap \<beta> M) = barriers \<beta>"
+proof -
+  have "finite (rd \<beta>)" by auto
+  thus ?thesis unfolding smap_def by auto
+qed
+
+lemma smap_empty [simp]:
+  "smap \<beta> Map.empty = \<beta>"
+proof -
+  have "finite (rd \<beta>)" by auto
+  thus ?thesis using smap1_fold_empty unfolding smap_def by auto
+qed
+
+lemma smap_rep [simp]:
+  "smap1 M x (smap \<beta> M) = smap \<beta> M"
+proof (cases "x \<in> rd \<beta>")
+  case True
+  have "Finite_Set.fold (smap1 M) \<beta> (insert x (rd \<beta>)) =
+        smap1 M x (Finite_Set.fold (smap1 M) \<beta> (rd \<beta>))"
+    using cfi.fold_insert_idem by blast
+  moreover have "insert x (rd \<beta>) = rd \<beta>" using True by auto
+  ultimately show ?thesis unfolding smap_def by auto
+next
+  case False
+  thus ?thesis by simp
+qed
+
+subsection \<open>forall Theories\<close>
+
+lemma forall_rd [simp]:
+  "\<forall>\<alpha> \<in> forall V \<beta>. rd \<alpha> = rd \<beta> - V"
+  unfolding forall_def by auto
+
+lemma forall_wr [simp]:
+  "\<forall>\<alpha> \<in> forall V \<beta>. wr \<alpha> = wr \<beta>"
+  unfolding forall_def by auto
+
+lemma forall_barriers [simp]:
+  "\<forall>\<alpha> \<in> forall V \<beta>. barriers \<alpha> = barriers \<beta>"
+  unfolding forall_def by auto
+
+lemma forall_fence [simp]:
+  "\<forall>\<alpha> \<in> forall V \<beta>.  (\<alpha> \<noteq> full_fence) = (\<beta> \<noteq> full_fence)"
+proof -
+  have "\<forall>\<alpha>. barriers \<alpha> = (\<alpha> = full_fence)" by (intro allI, case_tac \<alpha>; auto)
+  thus ?thesis using forall_barriers by blast
+qed
+
+lemma forall_nil [simp]:
+  "forall {} \<alpha> = {\<alpha>}"
+  unfolding forall_def by auto
+
+lemma smap1_cong [intro]:
+  "M x = N x \<Longrightarrow> smap1 M x = smap1 N x"
+  unfolding smap1_def using domIff by fastforce
+
+lemma
+  "comp_fun_commute_on (rd \<alpha>) (smap1 (\<lambda>y. if x = y then None else M y))"
+  by (rule Finite_Set.comp_fun_commute_on.intro) auto
+
+lemma
+  "comp_fun_commute_on (rd \<alpha>) (smap1 (\<lambda>y. if x = y then None else M y))"
+  by (rule Finite_Set.comp_fun_commute_on.intro) auto
+  
+lemma forall_unfold:
+  shows "forall (insert x V) \<alpha> = {subst\<^sub>i \<alpha>' x (Val c) | c \<alpha>'. \<alpha>' \<in> forall V \<alpha>}" (is "?L = ?R")
+proof -
+  have "?L \<subseteq> ?R"
+  proof (clarsimp simp: forall_def, cases "x \<in> V")
+    fix M assume d: "dom (M :: ('b, 'c) var \<Rightarrow> 'a option) = insert x V" "x \<in> V"
+    hence "smap \<alpha> M = subst\<^sub>i (smap \<alpha> M) x (Val (the (M x)))" by simp
+    moreover have "dom M = V" using d by auto
+    ultimately show "\<exists>c \<alpha>'. smap \<alpha> M = subst\<^sub>i \<alpha>' x (Val c) \<and> (\<exists>M. \<alpha>' = smap \<alpha> M \<and> dom M = V)"
+      by blast
+  next
+    fix M assume d: "dom (M :: ('b, 'c) var \<Rightarrow> 'a option) = insert x V" "x \<notin> V"
+    let ?M = "\<lambda>y. if x = y then None else M y"
+    have "smap \<alpha> M = subst\<^sub>i (smap \<alpha> ?M) x (Val (the (M x)))"
+    proof -
+      have 
+        "comp_fun_commute_on (rd \<alpha>) (smap1 M)" 
+        "comp_fun_commute_on (rd \<alpha>) (smap1 (\<lambda>y. if x = y then None else M y))"
+        by standard auto
+      hence mx: "Finite_Set.fold (smap1 M) \<alpha> (rd \<alpha> - {x}) = Finite_Set.fold (smap1 ?M) \<alpha> (rd \<alpha> - {x})"
+        by (auto intro!: Finite_Set.fold_cong simp add: cfi.comp_fun_commute_axioms)
+      show ?thesis
+      proof (cases "x \<in> rd \<alpha>")
+        case True
+        hence [simp]: "insert x (rd \<alpha>) = rd \<alpha>" by auto
+        have fx: "Finite_Set.fold (smap1 M) \<alpha> (insert x (rd \<alpha>)) = 
+                  smap1 M x (Finite_Set.fold (smap1 M) \<alpha> (rd \<alpha> - {x}))"
+          by (rule cfi.fold_insert_remove) blast
+        have "Finite_Set.fold (smap1 ?M) \<alpha> (insert x (rd \<alpha>)) = 
+                  smap1 ?M x (Finite_Set.fold (smap1 ?M) \<alpha> (rd \<alpha> - {x}))"
+          by (rule cfi.fold_insert_remove) blast
+        also have "... = Finite_Set.fold (smap1 ?M) \<alpha> (rd \<alpha> - {x})" by auto
+        finally show ?thesis using fx mx unfolding smap_def apply simp
+          unfolding smap1_def using d(1) by (auto split: if_splits)
+      next
+        case False
+        hence [simp]: "rd \<alpha> - {x} = rd \<alpha>" by auto
+        have "x \<notin> rd (smap \<alpha> ?M)" using False by simp
+        then show ?thesis using mx unfolding smap_def by simp
+      qed
+    qed
+    moreover have "dom ?M = V" using d by (auto split: if_splits)
+    ultimately show "\<exists>c \<alpha>'. smap \<alpha> M = subst\<^sub>i \<alpha>' x (Val c) \<and> (\<exists>M. \<alpha>' = smap \<alpha> M \<and> dom M = V)"
+      by blast
+  qed
+
+  moreover have "?R \<subseteq> ?L"
+  proof (clarsimp simp: forall_def, cases "x \<in> V")
+    fix M c assume d: "V = dom (M :: ('b, 'c) var \<Rightarrow> 'a option)" "x \<in> V" 
+    have "dom M = insert x (dom M)" using d by auto
+    moreover have "subst\<^sub>i (smap \<alpha> M) x (Val c) = smap \<alpha> M" using d by simp
+    ultimately show "\<exists>Ma. subst\<^sub>i (smap \<alpha> M) x (Val c) = smap \<alpha> Ma \<and> dom Ma = insert x (dom M)"
+      by blast
+  next
+    fix M c assume d: "V = dom (M :: ('b, 'c) var \<Rightarrow> 'a option)" "x \<notin> V" 
+    let ?M = "\<lambda>y. if y = x then Some c else M y"
+    have "dom ?M = insert x (dom M)" using d by auto
+    moreover have "subst\<^sub>i (smap \<alpha> M) x (Val c) = smap \<alpha> ?M"
+    proof -
+      have 
+        "comp_fun_commute_on (rd \<alpha>) (smap1 M)" 
+        "comp_fun_commute_on (rd \<alpha>) (smap1 (\<lambda>y. if y = x then Some c else M y))"
+        by standard auto
+      hence mx: "Finite_Set.fold (smap1 M) \<alpha> (rd \<alpha> - {x}) = Finite_Set.fold (smap1 ?M) \<alpha> (rd \<alpha> - {x})"
+        by (auto intro!: Finite_Set.fold_cong simp add: cfi.comp_fun_commute_axioms)
+      show ?thesis
+      proof (cases "x \<in> rd \<alpha>")
+        case True
+        hence [simp]: "insert x (rd \<alpha>) = rd \<alpha>" by auto
+        have fx: "Finite_Set.fold (smap1 ?M) \<alpha> (insert x (rd \<alpha>)) = 
+                  smap1 ?M x (Finite_Set.fold (smap1 ?M) \<alpha> (rd \<alpha> - {x}))"
+          by (rule cfi.fold_insert_remove) blast
+        have "Finite_Set.fold (smap1 M) \<alpha> (insert x (rd \<alpha>)) = 
+                  smap1 M x (Finite_Set.fold (smap1 M) \<alpha> (rd \<alpha> - {x}))"
+          by (rule cfi.fold_insert_remove) blast
+        also have "... = Finite_Set.fold (smap1 M) \<alpha> (rd \<alpha> - {x})" using d by auto        
+        finally show ?thesis using fx mx unfolding smap_def apply simp
+          unfolding smap1_def using d(1) by (auto split: if_splits)
+      next
+        case False
+        hence [simp]: "rd \<alpha> - {x} = rd \<alpha>" by auto
+        have "x \<notin> rd (smap \<alpha> ?M)" using False by simp
+        then show ?thesis using mx unfolding smap_def by simp
+      qed
+    qed
+    ultimately show "\<exists>Ma. subst\<^sub>i (smap \<alpha> M) x (Val c) = smap \<alpha> Ma \<and> dom Ma = insert x (dom M)"
+      by blast
+  qed
+
+  ultimately show ?thesis by blast
+qed
+
+lemma forall_one [simp]:
+  "forall {x} \<alpha> = {subst\<^sub>i \<alpha> x (Val c) | c. True}"
+  unfolding forall_unfold[of x "{}" \<alpha>] by auto
+
+lemma forall_nop [simp]:
+  assumes "x \<notin> rd \<alpha>" 
+  shows "forall (insert x V) \<alpha> = forall V \<alpha>"
+  using assms forall_unfold by force
+
+lemma forallI [intro]:
+  "smap \<alpha> M \<in> forall (dom M) \<alpha>"
+  by (auto simp: forall_def)
+
+(*end *)(*of locale *)
 
 end
 
 
+
+(*todo: smap1 lemmas only needed for static analysis part (to compute reorderable pairs?)
+        leave for now  *)
+
+(*
+lemma beh_smap1 [simp]:
+  "beh\<^sub>i (smap1 M x \<alpha>) = {(t,updTree (wr \<alpha>) (lookupSome t') t) |t t'.
+                           (updTree_part ({x} \<inter> dom M) (M) t,t') \<in> beh\<^sub>i \<alpha>}"
+(*  apply (cases \<alpha> ; auto simp: smap1_def updTree_def updTree_part_def) *)
+proof (cases \<alpha>)
+  case (assign x11 x12)
+  then show ?thesis sorry
+next
+  case (cmp b)
+  then show ?thesis 
+  proof -
+    have a0:"smap1 M x (cmp b) = (if x \<in> dom M then subst\<^sub>i (cmp b) x (Val (the (M x))) else (cmp b))"
+       using smap1_def cmp by blast
+     then have a1:"beh\<^sub>i (smap1 M x (cmp b)) = 
+         {(t,t'). t=t' \<and> ev\<^sub>B t (if (x \<in> dom M) then (subst\<^sub>B b x (Val(the (M x)))) else b)}" 
+      using smap1_def beh\<^sub>i.simps(2) subst\<^sub>i.simps(2) cmp by force
+    then have a2:"... = {(t,t)| t . ev\<^sub>B t (if (x \<in> dom M) then (subst\<^sub>B b x (Val(the (M x)))) else b)}"
+      using a1 by blast
+    have b0:"wr(cmp b) = {}" by simp
+    have b1:"\<forall> t t'. updTree (wr (cmp b)) (lookupSome t') t = t" using updTree_def b0 by simp
+    then have b2:"{(t,updTree(wr(cmp b))(lookupSome t') t)|t t'.
+                                  (updTree_part ({x} \<inter> dom M) M t, t') \<in> beh\<^sub>i (cmp b)} = 
+                    {(t,t)| t t'. (updTree_part ({x} \<inter> dom M) M t, t') \<in> beh\<^sub>i (cmp b)}" 
+      using b1 by simp
+    then have b3:"... = {(t,t)| t. ev\<^sub>B (updTree_part ({x} \<inter> dom M) M t) b}" using b2 beh\<^sub>i.simps(2) 
+         by simp
+    then have b4:"... = {(t,t)| t . ev\<^sub>B t (if (x \<in> dom M) then (subst\<^sub>B b x (Val(the (M x)))) else b)}"
+      using ev_updTreePart sorry
+    then show ?thesis using a0 a1 a2 b1 b2 b3 cmp by (smt (verit, del_insts) Collect_cong)
+  qed
+qed auto
+*)
+
+(*
+
+lemma beh_fold_smap1:
+  assumes "finite F" 
+  shows "beh\<^sub>i (Finite_Set.fold (smap1 M) \<alpha> F) = {(m\<^sub>1, upd_part (wr \<alpha>) (st m) m\<^sub>1) |m m\<^sub>1. (upd (F \<inter> dom M) (the \<circ> M) m\<^sub>1, m) \<in> beh\<^sub>i \<alpha>}"
+  using assms
+proof (induct)
+  case empty
+  then show ?case apply (cases \<alpha> ; auto) sorry
+next
+  case (insert x F)
+  hence f: "Finite_Set.fold (smap1 M) \<alpha> (insert x F) = 
+         smap1 M x (Finite_Set.fold (smap1 M) \<alpha> F)"
+    using cfi.fold_insert_idem by blast
+
+  show ?case using insert(1)
+    unfolding f beh_smap1 insert(3)
+    apply auto unfolding o_def 
+    apply (intro exI conjI)
+    apply blast
+    sorry
+(*  
+  apply (metis Int_Un_distrib2 Un_insert_right inf_bot_right sup_inf_absorb)
+    apply (intro exI conjI)
+    prefer 2
+    apply blast
+    apply simp
+    apply (metis Int_Un_distrib2 Un_insert_right inf_bot_right sup_inf_absorb)
+    done
+*)
+qed
+
+
+lemma beh_smap [simp]:
+  "beh\<^sub>i (smap \<alpha> M) = {(m\<^sub>1,upd_part (wr \<alpha>) (st m) m\<^sub>1) | m m\<^sub>1. (upd (dom M) (the o M) m\<^sub>1,m) \<in> beh\<^sub>i \<alpha>}"
+proof -
+  have "finite (rd \<alpha>)" by auto
+  hence "beh\<^sub>i (Finite_Set.fold (smap1 M) \<alpha> (rd \<alpha>)) = 
+          {(m\<^sub>1, upd_part (wr \<alpha>) (st m) m\<^sub>1) |m m\<^sub>1. (upd ((rd \<alpha>) \<inter> dom M) (the \<circ> M) m\<^sub>1, m) \<in> beh\<^sub>i \<alpha>}"
+    using beh_fold_smap1 by blast
+
+  also have "... = {(m\<^sub>1, upd_part (wr \<alpha>) (st m) m\<^sub>1) |m m\<^sub>1. (upd (dom M) (the \<circ> M) m\<^sub>1, m) \<in> beh\<^sub>i \<alpha>}"
+    apply (cases \<alpha>; auto)
+ sorry
+  finally show ?thesis unfolding smap_def .
+qed
+*)
