SimAsm/State2.thy
@@ -4,7 +4,7 @@ begin
 
 locale state = 
   fixes st :: "'s \<Rightarrow> 'var \<Rightarrow> 'val option"
-  fixes st_upd :: "'s \<Rightarrow> 'var \<Rightarrow> 'val \<Rightarrow> 's" ("_'((2_/ :=\<^sub>s/ _)')" [900,0,0] 901)
+  fixes st_upd :: "'s \<Rightarrow> 'var \<Rightarrow> 'val \<Rightarrow> 's" ("_'((2_/ :=\<^sub>u/ _)')" [900,0,0] 901)
   fixes aux :: "'sub \<Rightarrow> 'a"
   fixes aux_upd :: "'s \<Rightarrow> ('sub \<Rightarrow> 'a) \<Rightarrow> 's" ("_'((2aux:/ _)')" [900,0] 901)
   fixes aux_extract :: "'s \<Rightarrow> 'sub"
@@ -32,18 +32,18 @@ lemma st_upd_diff: "var2 \<noteq> var \<Longrightarrow> st (st_upd s var val) va
   using st_upd by auto
 
 lemma st_upd_fun [simp]:
-  "st (m(r :=\<^sub>s e)) = (\<lambda>x. (if r = x then Some e else st m x))"
+  "st (m(r :=\<^sub>u e)) = (\<lambda>x. (if r = x then Some e else st m x))"
   using st_upd by auto
 
 lemma st_upd_map:
-  "(\<lambda>v. st (t(x :=\<^sub>s e)) v) = (\<lambda>v. st t v)(x \<mapsto> e)"
+  "(\<lambda>v. st (t(x :=\<^sub>u e)) v) = (\<lambda>v. st t v)(x \<mapsto> e)"
   using st_upd_fun
   by auto
 
-lemma st_upd_twist: "a \<noteq> c \<Longrightarrow> m(a:=\<^sub>sb)(c:=\<^sub>sd) =\<^sub>s m(c:=\<^sub>sd)(a:=\<^sub>sb)"
+lemma st_upd_twist: "a \<noteq> c \<Longrightarrow> m(a:=\<^sub>ub)(c:=\<^sub>ud) =\<^sub>s m(c:=\<^sub>ud)(a:=\<^sub>ub)"
   by auto
 
-lemma st_upd_region: "region r \<noteq> region r2 \<Longrightarrow> st (m(r :=\<^sub>s e)) r2 = st m r2"
+lemma st_upd_region: "region r \<noteq> region r2 \<Longrightarrow> st (m(r :=\<^sub>u e)) r2 = st m r2"
   by auto
 
 lemma aux_exec': 
